\Kw{$C_k^{i-1} = \{ s_{k(1)}, \ldots, s_{k(r)}\}$}
\Begin{
  $C_k^i \gets \{s_{k(1)}\}$\;
  \For{$h \gets 2, r$}{
    $C_k^i = \{s_{\til{k}(1)}, \ldots, s_{\til{k}(l_h)}\}$\;
    $dominated \gets false$\;
    $dominates \gets false$\;
    $j \gets 1$\;
    \While{$ j \leq l_h$ \textbf{and} $\neg dominated$ \textbf{and} $\neg dominates$}{
      \uIf{$s_{\til{k}(j)} \rel_k^i s_{k(h)}$}{
        $dominated \gets true$\;
      }
      \ElseIf{$s_{k(h)} \rel_k^i s_{\til{k}(j)}$}{
        $C_k^i \gets C_k^i\backslash\{s_{\til{k}(j)}\}$\;
        $dominates \gets true$\;
      }
      $j \gets j + 1$\;
    }
    \If{$\neg dominated$}{
      \While{$j \leq l_h$}{
        \If{$s_{k(h)} \rel_k^i s_{\til{k}(j)}$}{
          $C_k^i \gets C_k^i \backslash \{s_{\til{k}(j)}\}$\;
        }
        $j \gets j + 1;$
      }
      $C_k^i \gets C_k^i \cup \{s_{k(h)}\};$
    }
  }
  \textbf{return} $C_k$
}